src/RationalTrees/RationalTree.v
@@ -11,6 +11,51 @@ Import EqNotations.
 Require Import Unification.
 
 
+(* Utils *)
+
+Polymorphic Fixpoint n_options (T : Type) (n : nat) : Type :=
+match n with
+| 0 => T
+| S n => option (n_options T n)
+end.
+
+Polymorphic Fixpoint map_filter [T R] (f : T -> option R) (xs : list T) : list R :=
+match xs with
+| nil => nil
+| x::xs =>
+  match f x with
+  | None => map_filter f xs
+  | Some x => x :: map_filter f xs
+  end
+end.
+
+Polymorphic Lemma map_filter_map_l [T S R] (f : S -> R) (g : T -> option S) xs
+                                 : map f (map_filter g xs)
+                                 = map_filter (fun x => option_map f (g x)) xs.
+Proof.
+  induction xs as [ | x xs ]. auto.
+  simpl. destruct (g x) as [ y | ]; auto. simpl. f_equal. apply IHxs.
+Qed.
+
+Polymorphic Lemma map_filter_map_r [T S R] (f : S -> option R) (g : T -> S) xs
+                                 : map_filter f (map g xs) = map_filter (fun x => f (g x)) xs.
+Proof. induction xs as [ | x xs ]. auto. simpl. rewrite IHxs. auto. Qed.
+
+Polymorphic Lemma map_filter_In [T R] (f : T -> option R) xs y
+                              : In y (map_filter f xs) <-> exists x, In x xs /\ f x = Some y.
+Proof.
+  constructor; intro.
+  * induction xs as [ | x xs ]. inversion H. simpl in H.
+    remember (f x) as res. symmetry in Heqres. destruct res as [ z | ]. destruct H.
+    - subst z. eexists. constructor; eauto. left. auto.
+    - apply IHxs in H. destruct H as [ x' [ H1 H2 ] ]. eexists. simpl. constructor; eauto.
+    - apply IHxs in H. destruct H as [ x' [ H1 H2 ] ]. eexists. simpl. constructor; eauto.
+  * destruct H as [ x' [ H1 H2 ] ]. induction xs as [ | x xs ]. inversion H1. destruct H1.
+    - subst x'. simpl. rewrite H2. left. auto.
+    - apply IHxs in H. simpl. destruct (f x); simpl; auto.
+Qed.
+
+
 (* Infinite Term *)
 
 CoInductive inf_term : Set :=
@@ -53,28 +98,47 @@ match p with
 end.
 
 CoFixpoint inf_term_eq_trans {t1 t2 t3} (p : inf_term_eq t1 t2) (q : inf_term_eq t2 t3)
-                             : inf_term_eq t1 t3.
-Proof.
-  refine (
-    match p in inf_term_eq t1' t2' return inf_term_eq t2' t3 -> inf_term_eq t1' t3 with
-    | VarInfEq n => fun q =>
-      match q with
-      | VarInfEq _ => VarInfEq _
-      end
-    | CstInfEq n => fun q =>
-      match q with
-      | CstInfEq _ => CstInfEq _
-      end
-    | ConInfEq n l1 l2 r1 r2 pl pr => fun q => _
-    end q
-  ).
-  good_inversion q.
-  refine (ConInfEq n l1 l3 r1 r3 (inf_term_eq_trans _ _ _ pl H3) (inf_term_eq_trans _ _ _ pr H4)).
-Defined.
+                             : inf_term_eq t1 t3 :=
+match p in inf_term_eq t1' t2' return inf_term_eq t2' t3 -> inf_term_eq t1' t3 with
+| VarInfEq n => fun q =>
+  match q with
+  | VarInfEq _ => VarInfEq _
+  end
+| CstInfEq n => fun q =>
+  match q with
+  | CstInfEq _ => CstInfEq _
+  end
+| ConInfEq n l1 l2 r1 r2 pl pr => fun q =>
+  match q in inf_term_eq t2' t3'
+  return ConInf n l2 r2 = t2' -> inf_term_eq (ConInf n l1 r1) t3'
+  with
+  | VarInfEq _ => fun p => match p with end
+  | CstInfEq _ => fun p => match p with end
+  | ConInfEq n' l2' l3 r2' r3 pl' pr' => fun p =>
+    let pn : n = n' := match p in _ = ConInf n' _ _ return n = n' with
+    | eq_refl => eq_refl
+    end in
+    let pl2 : l2' = l2 := match p in _ = ConInf _ l2' _ return l2' = l2 with
+    | eq_refl => eq_refl
+    end in
+    let pr2 : r2' = r2 := match p in _ = ConInf _ _ r2' return r2' = r2 with
+    | eq_refl => eq_refl
+    end in
+    rew [fun x => inf_term_eq _ (ConInf x _ _)] pn in ConInfEq n l1 l3 r1 r3
+    (inf_term_eq_trans pl (rew [fun x => inf_term_eq x _] pl2 in pl'))
+    (inf_term_eq_trans pr (rew [fun x => inf_term_eq x _] pr2 in pr'))
+  end eq_refl
+end q.
 
 Instance inf_term_eq_equivalence : RelationClasses.Equivalence inf_term_eq :=
   RelationClasses.Build_Equivalence _ inf_term_eq_refl (fun _ _ => inf_term_eq_sym)
     (fun _ _ _ => inf_term_eq_trans).
+
+CoInductive is_inf_term_FV (x : name) : inf_term -> Prop :=
+| VarInfFV : is_inf_term_FV x (VarInf x)
+| ConInfFVL n l r : is_inf_term_FV x l -> is_inf_term_FV x (ConInf n l r)
+| ConInfFVR n l r : is_inf_term_FV x r -> is_inf_term_FV x (ConInf n l r)
+.
 
 Definition inf_subst : Set := name -> inf_term.
 
@@ -109,6 +173,26 @@ match t as t' return inf_term_eq (inf_term_step (apply_inf_subst inf_subst_trivi
 | ConInf n l r => ConInfEq n _ _ _ _ (apply_inf_subst_trivial l) (apply_inf_subst_trivial r)
 end.
 
+CoFixpoint apply_inf_subst_ext s1 s2 t
+                               (p : forall n, is_inf_term_FV n t -> inf_term_eq (s1 n) (s2 n))
+                             : inf_term_eq (apply_inf_subst s1 t) (apply_inf_subst s2 t) :=
+rew <- [fun x => inf_term_eq x _] inf_term_step_prop (apply_inf_subst s1 t) in
+rew <- [fun x => inf_term_eq _ x] inf_term_step_prop (apply_inf_subst s2 t) in
+match t as t'
+return (forall n, is_inf_term_FV n t' -> inf_term_eq (s1 n) (s2 n))
+    -> inf_term_eq (inf_term_step (apply_inf_subst s1 t'))
+                   (inf_term_step (apply_inf_subst s2 t'))
+with
+| VarInf n => fun p =>
+  rew [fun x => inf_term_eq x _] inf_term_step_prop (s1 n) in
+  rew [fun x => inf_term_eq _ x] inf_term_step_prop (s2 n) in
+  p n (VarInfFV _)
+| CstInf n => fun _ => CstInfEq _
+| ConInf n l r => fun p => ConInfEq n _ _ _ _
+  (apply_inf_subst_ext s1 s2 l (fun n' p' => p n' (ConInfFVL _ _ _ _ p')))
+  (apply_inf_subst_ext s1 s2 r (fun n' p' => p n' (ConInfFVR _ _ _ _ p')))
+end p.
+
 Definition inf_subst_compose (s1 s2 : inf_subst) : inf_subst :=
   fun n => apply_inf_subst s1 (s2 n).
 
@@ -131,32 +215,6 @@ with
 | ConInf n l r =>
   ConInfEq n _ _ _ _ (inf_subst_compose_prop s1 s2 l) (inf_subst_compose_prop s1 s2 r)
 end.
-
-CoInductive is_inf_term_FV (x : name) : inf_term -> Prop :=
-| VarInfFV : is_inf_term_FV x (VarInf x)
-| ConInfFVL n l r : is_inf_term_FV x l -> is_inf_term_FV x (ConInf n l r)
-| ConInfFVR n l r : is_inf_term_FV x r -> is_inf_term_FV x (ConInf n l r)
-.
-
-CoFixpoint apply_inf_subst_ext s1 s2 t
-                               (p : forall n, is_inf_term_FV n t -> inf_term_eq (s1 n) (s2 n))
-                             : inf_term_eq (apply_inf_subst s1 t) (apply_inf_subst s2 t) :=
-rew <- [fun x => inf_term_eq x _] inf_term_step_prop (apply_inf_subst s1 t) in
-rew <- [fun x => inf_term_eq _ x] inf_term_step_prop (apply_inf_subst s2 t) in
-match t as t'
-return (forall n, is_inf_term_FV n t' -> inf_term_eq (s1 n) (s2 n))
-    -> inf_term_eq (inf_term_step (apply_inf_subst s1 t'))
-                   (inf_term_step (apply_inf_subst s2 t'))
-with
-| VarInf n => fun p =>
-  rew [fun x => inf_term_eq x _] inf_term_step_prop (s1 n) in
-  rew [fun x => inf_term_eq _ x] inf_term_step_prop (s2 n) in
-  p n (VarInfFV _)
-| CstInf n => fun _ => CstInfEq _
-| ConInf n l r => fun p => ConInfEq n _ _ _ _
-  (apply_inf_subst_ext s1 s2 l (fun n' p' => p n' (ConInfFVL _ _ _ _ p')))
-  (apply_inf_subst_ext s1 s2 r (fun n' p' => p n' (ConInfFVR _ _ _ _ p')))
-end p.
 
 Definition is_ground_inf_term (t : inf_term) : Prop := forall x, ~is_inf_term_FV x t.
 
@@ -351,6 +409,317 @@ Instance grt_eq_equivalence : RelationClasses.Equivalence grt_eq :=
 
 (* Mu-Term *)
 
+Inductive mu_term' (V : Set) : Set :=
+| VarMu' : V -> mu_term' V
+| CstMu' : name -> mu_term' V
+| ConMu' : name -> mu_term' V -> mu_term' V -> mu_term' V
+| BndMu' : mu_term' (option V) -> mu_term' V
+.
+
+Arguments VarMu' [_] _.
+Arguments CstMu' [_] _.
+Arguments ConMu' [_] _ _ _.
+Arguments BndMu' [_] _.
+
+Fixpoint mu_term'_fv [V] (t : mu_term' V) : list V :=
+match t with
+| VarMu' n => [n]
+| CstMu' _ => []
+| ConMu' _ l r => mu_term'_fv l ++ mu_term'_fv r
+| BndMu' t => map_filter id (mu_term'_fv t)
+end.
+
+Fixpoint mu_term'_map [V U : Set] (f : V -> U) (t : mu_term' V) : mu_term' U :=
+match t with
+| VarMu' n => VarMu' (f n)
+| CstMu' n => CstMu' n
+| ConMu' n l r => ConMu' n (mu_term'_map f l) (mu_term'_map f r)
+| BndMu' t => BndMu' (mu_term'_map (option_map f) t)
+end.
+
+Lemma mu_term'_map_fv [V U : Set] (f : V -> U) t
+                    : mu_term'_fv (mu_term'_map f t) = map f (mu_term'_fv t).
+Proof.
+  generalize dependent U. induction t; simpl; intros; auto.
+  * rewrite IHt1, IHt2. symmetry. apply map_app.
+  * rewrite IHt. etransitivity. apply map_filter_map_r. symmetry.
+    etransitivity. apply map_filter_map_l. auto.
+Qed.
+
+Lemma mu_term'_map_ext [V U : Set] (f g : V -> U) t
+                     : (forall v, In v (mu_term'_fv t) -> f v = g v)
+                   <-> mu_term'_map f t = mu_term'_map g t.
+Proof.
+  constructor; intro.
+  * generalize dependent U. induction t; simpl; intros; f_equal.
+    - apply H. left. auto.
+    - apply IHt1. intros. apply H. apply in_app_iff. auto.
+    - apply IHt2. intros. apply H. apply in_app_iff. auto.
+    - apply IHt. intros. destruct v; simpl; f_equal. apply H.
+      apply map_filter_In. eexists. constructor; eauto.
+  * generalize dependent U. induction t; simpl; intros.
+    - destruct H0. good_inversion H. auto. inversion H0.
+    - inversion H0.
+    - good_inversion H. apply in_app_iff in H0. destruct H0.
+      apply IHt1; auto. apply IHt2; auto.
+    - good_inversion H. apply map_filter_In in H0. destruct H0 as [ x [ H0 H1 ] ].
+      unfold id in H1. subst x. eapply IHt in H2; eauto. simpl in H2. good_inversion H2. auto.
+Qed.
+
+Lemma mu_term'_map_inj [V U : Set] (f : V -> U) t1 t2
+                       (H1 : forall x y, f x = f y -> x = y)
+                       (H2 : mu_term'_map f t1 = mu_term'_map f t2)
+                     : t1 = t2.
+Proof.
+  generalize dependent t2. generalize dependent U.
+  induction t1; simpl; intros; destruct t2; good_inversion H2; simpl; f_equal; auto.
+  * eapply IHt1_1; eauto.
+  * eapply IHt1_2; eauto.
+  * eapply IHt1; eauto. intros. destruct x; destruct y; good_inversion H; f_equal.
+    apply H1. auto.
+Qed.
+
+Lemma mu_term'_map_map [V U W : Set] (f : U -> W) (g : V -> U) t
+                     : mu_term'_map f (mu_term'_map g t) = mu_term'_map (fun x => f (g x)) t.
+Proof.
+  generalize dependent W. generalize dependent U. induction t; simpl; intros; f_equal; auto.
+  etransitivity. apply IHt. apply mu_term'_map_ext. intros. destruct v; auto.
+Qed.
+
+Definition mu_term'_BndMu'_k [V U : Set] (k : V -> mu_term' U)
+                             (n : option V) : mu_term' (option U) :=
+match n with
+| None => VarMu' None
+| Some n => mu_term'_map Some (k n)
+end.
+
+Fixpoint mu_term'_bind [V U : Set] (k : V -> mu_term' U) (t : mu_term' V) : mu_term' U :=
+match t with
+| VarMu' n => k n
+| CstMu' n => CstMu' n
+| ConMu' n l r => ConMu' n (mu_term'_bind k l) (mu_term'_bind k r)
+| BndMu' t => BndMu' (mu_term'_bind (mu_term'_BndMu'_k k) t)
+end.
+
+Lemma mu_term'_bind_ext [V U : Set] (f g : V -> mu_term' U) t
+                      : (forall v, In v (mu_term'_fv t) -> f v = g v)
+                    <-> mu_term'_bind f t = mu_term'_bind g t.
+Proof.
+  constructor; intro.
+  * generalize dependent U. induction t; simpl; intros; auto; f_equal.
+    - apply IHt1. intros. apply H. apply in_app_iff. auto.
+    - apply IHt2. intros. apply H. apply in_app_iff. auto.
+    - apply IHt. intros. destruct v; simpl; f_equal.
+      apply H. apply map_filter_In. eexists. constructor; eauto.
+  * generalize dependent U. induction t; simpl; intros.
+    - destruct H0. subst. auto. inversion H0.
+    - inversion H0.
+    - good_inversion H. apply in_app_iff in H0. destruct H0.
+      apply IHt1; auto. apply IHt2; auto.
+    - good_inversion H. apply map_filter_In in H0. destruct H0 as [ x [ H0 H1 ] ].
+      unfold id in H1. subst x. eapply IHt in H2; eauto. simpl in H2.
+      apply mu_term'_map_inj in H2; auto. intros. good_inversion H. auto.
+Qed.
+
+Lemma mu_term'_bind_pure [V : Set] t : mu_term'_bind (VarMu' (V:=V)) t = t.
+Proof.
+  induction t; simpl; f_equal; auto. etransitivity; [ | eauto ].
+  apply mu_term'_bind_ext. intros. destruct v; auto.
+Qed.
+
+Lemma mu_term'_bind_map_r [V U W : Set] (k : U -> mu_term' W) (f : V -> U) t
+                        : mu_term'_bind k (mu_term'_map f t) = mu_term'_bind (fun x => k (f x)) t.
+Proof.
+  generalize dependent W. generalize dependent U. induction t; simpl; intros; f_equal; auto.
+  etransitivity. apply IHt. apply mu_term'_bind_ext. intros. destruct v; auto.
+Qed.
+
+Lemma mu_term'_bind_map_l [V U W : Set] (f : U -> W) (k : V -> mu_term' U) t
+                        : mu_term'_map f (mu_term'_bind k t)
+                        = mu_term'_bind (fun x => mu_term'_map f (k x)) t.
+Proof.
+  generalize dependent W. generalize dependent U. induction t; simpl; intros; f_equal; auto.
+  etransitivity. apply IHt. apply mu_term'_bind_ext. intros. destruct v; auto. simpl.
+  etransitivity. apply mu_term'_map_map. symmetry. etransitivity. apply mu_term'_map_map.
+  apply mu_term'_map_ext. intros. auto.
+Qed.
+
+Lemma mu_term'_bind_assoc [V U W : Set] (k1 : U -> mu_term' W) (k2 : V -> mu_term' U) t
+                        : mu_term'_bind k1 (mu_term'_bind k2 t)
+                        = mu_term'_bind (fun x => mu_term'_bind k1 (k2 x)) t.
+Proof.
+  generalize dependent W. generalize dependent U. induction t; simpl; intros; f_equal; auto.
+  etransitivity. apply IHt. apply mu_term'_bind_ext. intros. destruct v; auto. simpl.
+  etransitivity. apply mu_term'_bind_map_r. symmetry. etransitivity. apply mu_term'_bind_map_l.
+  apply mu_term'_bind_ext. intros. auto.
+Qed.
+
+(* Actually, we only need to forbid (mu x. x) because of interpretation inexistence,
+ * but in practice it's convenient to allow only constructor inside of binder
+ * since all other legal mu-terms can be easily converted to the corresponding form
+ *)
+Inductive mu_term_wf' [V] : mu_term' V -> Prop :=
+| VarMuWF' n : mu_term_wf' (VarMu' n)
+| CstMuWF' n : mu_term_wf' (CstMu' n)
+| ConMuWF' n l r : mu_term_wf' l -> mu_term_wf' r -> mu_term_wf' (ConMu' n l r)
+| BndMuWF' n l r : mu_term_wf' (ConMu' n l r) -> mu_term_wf' (BndMu' (ConMu' n l r))
+.
+
+Lemma mu_term_wf'_ConMu_l [V] {n} {l r : mu_term' V}
+                          (H : mu_term_wf' (ConMu' n l r))
+                        : mu_term_wf' l.
+Proof. inversion H. auto. Qed.
+
+Lemma mu_term_wf'_ConMu_r [V] {n} {l r : mu_term' V}
+                          (H : mu_term_wf' (ConMu' n l r))
+                        : mu_term_wf' r.
+Proof. inversion H. auto. Qed.
+
+Lemma mu_term'_map_wf [V U : Set] (f : V -> U) {t} (H : mu_term_wf' t)
+                    : mu_term_wf' (mu_term'_map f t).
+Proof. generalize dependent U. induction H; simpl; intros; constructor; eauto. Qed.
+
+Lemma mu_term'_bind_wf [V U : Set] (k : V -> mu_term' U) {t}
+                       (H1 : forall n, mu_term_wf' (k n))
+                       (H2 : mu_term_wf' t)
+                     : mu_term_wf' (mu_term'_bind k t).
+Proof.
+  generalize dependent U. induction H2; simpl; intros; auto; constructor; auto.
+  apply IHmu_term_wf'. intros. destruct n0; [ | constructor ]. apply mu_term'_map_wf. auto.
+Qed.
+
+Definition mu_unfold_step'_k [V : Set] (t : mu_term' (option V)) (n : option V) : mu_term' V :=
+match n with
+| None => BndMu' t
+| Some n => VarMu' n
+end.
+
+Lemma mu_unfold_step'_k_bind [V U : Set] (k : V -> mu_term' U) (t1 : mu_term' (option V)) t2
+                           : mu_term'_bind k (mu_term'_bind (mu_unfold_step'_k t1) t2)
+                           = mu_term'_bind (mu_unfold_step'_k (mu_term'_bind (mu_term'_BndMu'_k k) t1))
+                                           (mu_term'_bind (mu_term'_BndMu'_k k) t2).
+Proof.
+  etransitivity. apply mu_term'_bind_assoc. symmetry.
+  etransitivity. apply mu_term'_bind_assoc. apply mu_term'_bind_ext.
+  intros. clear t2 H. destruct v; auto. simpl.
+  etransitivity. apply mu_term'_bind_map_r. symmetry.
+  etransitivity. symmetry. apply mu_term'_bind_pure.
+  apply mu_term'_bind_ext. intros. auto.
+Qed.
+
+Definition mu_unfold_step' [V : Set] (t : mu_term' (option V)) : mu_term' V :=
+  mu_term'_bind (mu_unfold_step'_k t) t.
+
+Lemma mu_unfold_step'_wf [V : Set] {t : mu_term' (option V)}
+                         (H : mu_term_wf' (BndMu' t))
+                       : mu_term_wf' (mu_unfold_step' t).
+Proof.
+  apply mu_term'_bind_wf.
+  * intro. destruct n. constructor. auto.
+  * inversion H. auto.
+Qed.
+
+Lemma mu_unfold_step_not_BndMu [V : Set] {t t' : mu_term' (option V)}
+                               (H : mu_term_wf' (BndMu' t))
+                             : mu_unfold_step' t <> BndMu' t'.
+Proof. unfold mu_unfold_step'. good_inversion H. simpl. intro. inversion H. Qed.
+
+Definition mu_unfold_hlp' (mu_unfold' : forall (t : mu_term' name), mu_term_wf' t -> inf_term)
+                          t (t' : mu_term' name) (H1 : mu_unfold_step' t = t')
+                          (H2 : mu_term_wf' (BndMu' t)) (H3 : mu_term_wf' t')
+                        : inf_term :=
+match t' as t'' return mu_term_wf' t'' -> mu_unfold_step' t = t'' -> _ with
+| VarMu' n => fun _ _ => VarInf n
+| CstMu' n => fun _ _ => CstInf n
+| ConMu' n l r => fun H3 _ =>
+  ConInf n (mu_unfold' l (mu_term_wf'_ConMu_l H3)) (mu_unfold' r (mu_term_wf'_ConMu_r H3))
+| BndMu' t' => fun _ H1 => False_rec _ (mu_unfold_step_not_BndMu H2 H1)
+end H3 H1.
+
+CoFixpoint mu_unfold' (t : mu_term' name) (H : mu_term_wf' t) : inf_term :=
+match t as t' return mu_term_wf' t' -> _ with
+| VarMu' n => fun _ => VarInf n
+| CstMu' n => fun _ => CstInf n
+| ConMu' n l r => fun H =>
+  ConInf n (mu_unfold' l (mu_term_wf'_ConMu_l H)) (mu_unfold' r (mu_term_wf'_ConMu_r H))
+| BndMu' t => fun H => mu_unfold_hlp' mu_unfold' t _ eq_refl H (mu_unfold_step'_wf H)
+end H.
+
+CoFixpoint mu_unfold'_irrelevance t H1 H2 : inf_term_eq (mu_unfold' t H1) (mu_unfold' t H2) :=
+rew <- [fun x => inf_term_eq x _] inf_term_step_prop (mu_unfold' t H1) in
+rew <- [fun x => inf_term_eq _ x] inf_term_step_prop (mu_unfold' t H2) in
+match t as t'
+return forall H1 H2, inf_term_eq (inf_term_step (mu_unfold' t' H1))
+                                 (inf_term_step (mu_unfold' t' H2))
+with
+| VarMu' n => fun _ _ => VarInfEq n
+| CstMu' n => fun _ _ => CstInfEq n
+| ConMu' n l r => fun H1 H2 =>
+  ConInfEq n _ _ _ _ (mu_unfold'_irrelevance _ _ _) (mu_unfold'_irrelevance _ _ _)
+| BndMu' t => fun H1 H2 =>
+  rew [fun x => inf_term_eq x _] inf_term_step_prop (mu_unfold_hlp' mu_unfold' t _ _ H1 _) in
+  rew [fun x => inf_term_eq _ x] inf_term_step_prop (mu_unfold_hlp' mu_unfold' t _ _ H2 _) in
+  match mu_unfold_step' t as t'
+  return forall p H1' H2', inf_term_eq (mu_unfold_hlp' mu_unfold' t t' p H1 H1')
+                                       (mu_unfold_hlp' mu_unfold' t t' p H2 H2')
+  with
+  | VarMu' n' => fun _ _ _ => VarInfEq n'
+  | CstMu' n' => fun _ _ _ => CstInfEq n'
+  | ConMu' n' l r => fun _ H1' H2' =>
+    ConInfEq n' _ _ _ _ (mu_unfold'_irrelevance _ _ _) (mu_unfold'_irrelevance _ _ _)
+  | BndMu' t' => fun p _ _ => False_ind _ (mu_unfold_step_not_BndMu H1 p)
+  end eq_refl _ _
+end H1 H2.
+
+CoFixpoint mu_unfold'_bind k t (H1 : mu_term_wf' t)
+                           (H2 : mu_term_wf' (mu_term'_bind k t))
+                           (H3 : forall x, mu_term_wf' (k x))
+                         : inf_term_eq (mu_unfold' (mu_term'_bind k t) H2)
+                                       (apply_inf_subst (fun x => mu_unfold' (k x) (H3 x))
+                                                        (mu_unfold' t H1)) :=
+rew <- [fun x => inf_term_eq x _] inf_term_step_prop (mu_unfold' (mu_term'_bind k t) H2) in
+rew <- [fun x => inf_term_eq _ x] inf_term_step_prop (apply_inf_subst _ (mu_unfold' t H1)) in
+match t as t'
+return forall H1 H2, inf_term_eq (inf_term_step (mu_unfold' (mu_term'_bind k t') H2))
+                                 (inf_term_step (apply_inf_subst (fun x => mu_unfold' (k x) (H3 x))
+                                                                 (mu_unfold' t' H1)))
+with
+| VarMu' n => fun H1 H2 =>
+  rew [fun x => inf_term_eq x _] inf_term_step_prop (mu_unfold' (k n) H2) in
+  rew [fun x => inf_term_eq _ x] inf_term_step_prop (mu_unfold' (k n) (H3 n)) in
+  mu_unfold'_irrelevance (k n) H2 (H3 n)
+| CstMu' n => fun _ _ => CstInfEq n
+| ConMu' n l r => fun H1 H2 =>
+  ConInfEq n _ _ _ _ (mu_unfold'_bind k l _ _ _) (mu_unfold'_bind k r _ _ _)
+| BndMu' (ConMu' n l r) => fun H1 H2 => ConInfEq n _ _ _ _
+  ((
+    rew [fun x => forall (H2 : mu_term_wf' x), inf_term_eq (mu_unfold' _ H2) _]
+      mu_unfold_step'_k_bind k (ConMu' n l r) l
+    in
+    ((fun H2 => mu_unfold'_bind k _ _ H2 H3) : forall H2, inf_term_eq (mu_unfold' _ H2) _)
+  ) _)
+  ((
+    rew [fun x => forall (H2 : mu_term_wf' x), inf_term_eq (mu_unfold' _ H2) _]
+      mu_unfold_step'_k_bind k (ConMu' n l r) r
+    in
+    ((fun H2 => mu_unfold'_bind k _ _ H2 H3) : forall H2, inf_term_eq (mu_unfold' _ H2) _)
+  ) _)
+| BndMu' (VarMu' n) => fun H1 => False_rec _ (match H1 with end)
+| BndMu' (CstMu' n) => fun H1 => False_rec _ (match H1 with end)
+| BndMu' (BndMu' t) => fun H1 => False_rec _ (match H1 with end)
+end H1 H2.
+
+Corollary mu_unfold'_bind' k s t1 t2 (H1 : mu_term_wf' t1) (H2 : forall n, mu_term_wf' (k n))
+                           (H3 : inf_term_eq (mu_unfold' t1 H1) t2)
+                           (H4 : forall n, inf_term_eq (mu_unfold' (k n) (H2 n)) (s n))
+                           (H5 : mu_term_wf' (mu_term'_bind k t1))
+                         : inf_term_eq (mu_unfold' (mu_term'_bind k t1) H5) (apply_inf_subst s t2).
+Proof.
+  etransitivity. apply mu_unfold'_bind.
+  etransitivity. apply apply_inf_subst_eq. eauto.
+  apply apply_inf_subst_ext. intros. eauto.
+Qed.
+
 Inductive mu_term : Set :=
 | VarMu : name -> mu_term
 | CstMu : name -> mu_term
@@ -358,65 +727,57 @@ Inductive mu_term : Set :=
 | BndMu : name -> mu_term -> mu_term
 .
 
-Fixpoint mu_subst (x : name) (t' t : mu_term) : mu_term :=
+Definition mu_term_to_mu_term'_f (n n' : name) : option name :=
+  if name_eq_dec n n' then None else Some n'.
+
+Fixpoint mu_term_to_mu_term' (t : mu_term) : mu_term' name :=
 match t with
-| VarMu n => if name_eq_dec x n then t' else VarMu n
-| CstMu n => CstMu n
-| ConMu n l r => ConMu n (mu_subst x t' l) (mu_subst x t' r)
-| BndMu n t => if name_eq_dec x n then BndMu n t else BndMu n (mu_subst x t' t)
+| VarMu n => VarMu' n
+| CstMu n => CstMu' n
+| ConMu n l r => ConMu' n (mu_term_to_mu_term' l) (mu_term_to_mu_term' r)
+| BndMu n t => BndMu' (mu_term'_map (mu_term_to_mu_term'_f n) (mu_term_to_mu_term' t))
 end.
 
-(* Actually, we only need to forbid (mu x. x) because of interpretation inexistence,
- * but in practice it's convenient to allow only constructor inside of binder
- * since all other legal mu-terms can be easily converted to the corresponding form
- *)
-Inductive mu_term_wf : mu_term -> Prop :=
-| VarMuWF n : mu_term_wf (VarMu n)
-| CstMuWF n : mu_term_wf (CstMu n)
-| ConMuWF n l r : mu_term_wf l -> mu_term_wf r -> mu_term_wf (ConMu n l r)
-| BndMuWF n1 n2 l r : mu_term_wf (ConMu n2 l r) -> mu_term_wf (BndMu n1 (ConMu n2 l r))
-.
+Fixpoint mu_term_fv (t : mu_term) : var_set :=
+match t with
+| VarMu x => [x]
+| CstMu _ => []
+| ConMu _ l r => var_set_union (mu_term_fv l) (mu_term_fv r)
+| BndMu x t => var_set_remove x (mu_term_fv t)
+end.
 
-Lemma mu_term_wf_con_l {n l r} (twf : mu_term_wf (ConMu n l r)) : mu_term_wf l.
-Proof. inversion twf. auto. Qed.
-
-Lemma mu_term_wf_con_r {n l r} (twf : mu_term_wf (ConMu n l r)) : mu_term_wf r.
-Proof. inversion twf. auto. Qed.
-
-Lemma mu_subst_wf {n t' t} (twf' : mu_term_wf t') (twf : mu_term_wf t) : mu_term_wf (mu_subst n t' t).
+Lemma mu_term_fv_distinct t : NoDup (mu_term_fv t).
 Proof.
-  induction t; simpl; auto.
-  - destruct (name_eq_dec n n0); subst; auto.
-  - good_inversion twf. constructor; [ apply IHt1 | apply IHt2 ]; auto.
-  - destruct (name_eq_dec n n0). subst. auto. good_inversion twf.
-    specialize (IHt H0). good_inversion IHt. simpl. constructor. constructor; auto.
+  induction t; repeat constructor; auto.
+  * apply set_union_nodup; auto.
+  * apply set_remove_nodup. auto.
 Qed.
 
-Definition unfold_mu_step (n : name) (t : mu_term) : mu_term :=
-  mu_subst n (BndMu n t) t.
+Lemma mu_term_fv_prop t n : In n (mu_term_fv t) <-> In n (mu_term'_fv (mu_term_to_mu_term' t)).
+Proof.
+  induction t; simpl; try reflexivity.
+  * constructor; intro.
+    - apply in_app_iff. apply set_union_elim in H.
+      destruct H. apply IHt1 in H. auto. apply IHt2 in H. auto.
+    - apply in_app_iff in H. apply set_union_intro.
+      destruct H. apply IHt1 in H. auto. apply IHt2 in H. auto.
+  * constructor; intro.
+    - apply set_remove_iff in H; [ | apply mu_term_fv_distinct ]. destruct H.
+      apply map_filter_In. apply IHt in H. exists (Some n). constructor; auto.
+      rewrite mu_term'_map_fv. apply in_map_iff. eexists. constructor; eauto.
+      unfold mu_term_to_mu_term'_f. destruct (name_eq_dec n0 n); auto. exfalso. apply H0. auto.
+    - apply set_remove_iff. apply mu_term_fv_distinct. apply map_filter_In in H.
+      destruct H as [ x [ H1 H2 ] ]. unfold id in H2. subst x.
+      rewrite mu_term'_map_fv in H1. apply in_map_iff in H1.
+      destruct H1 as [ x [ H1 H2 ] ]. unfold mu_term_to_mu_term'_f in H1.
+      destruct (name_eq_dec n0 x); good_inversion H1. constructor; auto.
+      apply IHt. auto.
+Qed.
 
-Lemma unfold_mu_step_wf {n t} (twf : mu_term_wf (BndMu n t)) : mu_term_wf (unfold_mu_step n t).
-Proof. apply mu_subst_wf. auto. good_inversion twf. auto. Qed.
+Definition mu_term_wf (t : mu_term) : Prop := mu_term_wf' (mu_term_to_mu_term' t).
 
-Lemma unfold_mu_step_not_BndMu {n n' t t'} (twf : mu_term_wf (BndMu n t))
-                             : unfold_mu_step n t <> BndMu n' t'.
-Proof. unfold unfold_mu_step. good_inversion twf. simpl. intro. inversion H. Qed.
+Definition mu_unfold (t : mu_term) (H : mu_term_wf t) : inf_term :=
+  mu_unfold' (mu_term_to_mu_term' t) H.
 
-Definition unfold_mu_hlp (unfold_mu : forall t, mu_term_wf t -> inf_term)
-                         n t (twf : mu_term_wf (BndMu n t)) : inf_term :=
-match unfold_mu_step n t as t' return mu_term_wf t' -> unfold_mu_step n t = t' -> _ with
-| VarMu n => fun _ _ => VarInf n
-| CstMu n => fun _ _ => CstInf n
-| ConMu n l r => fun twf _ =>
-  ConInf n (unfold_mu l (mu_term_wf_con_l twf)) (unfold_mu r (mu_term_wf_con_r twf))
-| BndMu n' t' => fun _ p => False_rec _ (unfold_mu_step_not_BndMu twf p)
-end (unfold_mu_step_wf twf) eq_refl.
-
-CoFixpoint unfold_mu (t : mu_term) (twf : mu_term_wf t) : inf_term :=
-match t as t' return mu_term_wf t' -> _ with
-| VarMu n => fun _ => VarInf n
-| CstMu n => fun _ => CstInf n
-| ConMu n l r => fun twf =>
-  ConInf n (unfold_mu l (mu_term_wf_con_l twf)) (unfold_mu r (mu_term_wf_con_r twf))
-| BndMu n t => fun twf => unfold_mu_hlp unfold_mu n t twf
-end twf.
+Lemma mu_unfold_irrelevance t H1 H2 : inf_term_eq (mu_unfold t H1) (mu_unfold t H2).
+Proof. apply mu_unfold'_irrelevance. Qed.
